theories/iris/examples/effects/generator_client.v
@@ -19,6 +19,9 @@ Set Implicit Arguments.
 Unset Strict Implicit.
 Unset Printing Implicit Defensive.
 
+
+
+
 Definition naturals_type := Tf [] [].
 Definition cont_type := T_contref naturals_type.
 Definition sum_until_body_type := Tf [] [T_num T_i32].
@@ -42,8 +45,8 @@ Definition sum_until_client_neg :=
   [BI_const $ xx (-4294967293); BI_call 0].
 
 Section GeneratorClient.
-  Context `{!wasmG Σ, !hvisG Σ, !hmsG Σ, !hasG Σ}.
-  Context `{!inG Σ (excl_authR (listO (leibnizO i32)))}.
+  Context `{!wasmG Σ, !hvisG Σ, !hmsG Σ, !hasG Σ, !ghostG Σ}.
+  
 
   Definition sum_until_client tag_exp_addr generator_exp_addr sum_until_exp_addr mod_addr n :=
     [ ID_instantiate [ tag_exp_addr; generator_exp_addr; sum_until_exp_addr ] mod_addr [];
@@ -101,3 +104,145 @@ H_invoke sum_until_exp_addr [VAL_int32 n]
   Qed.
 
 End GeneratorClient.
+
+
+
+
+
+Section generator_client_adequacy.
+
+  Context (Σ: gFunctors).
+  Context {inv_preg: invGpreS Σ}.
+  Context {na_invg: na_invG Σ}.
+  Context {func_preg: gen_heapGpreS N function_closure Σ}.
+  Context {tab_preg: gen_heapGpreS (N*N) funcelem Σ}.
+  Context {tabsize_preg: gen_heapGpreS N nat Σ}.
+  Context {tablimits_preg: gen_heapGpreS N (option N) Σ}.
+  Context {mem_preg: gen_heapGpreS (N*N) byte Σ}.
+  Context {memsize_preg: gen_heapGpreS N N Σ}.
+  Context {memlimit_preg: gen_heapGpreS N (option N) Σ}.
+  Context {glob_preg: gen_heapGpreS N global Σ}.
+  Context {vis_preg: gen_heapGpreS N module_export Σ}.
+  Context {ms_preg: gen_heapGpreS N module Σ}.
+  Context {has_preg: gen_heapGpreS N host_action Σ}.
+  Context {tag_preg: gen_heapGpreS N function_type Σ}.
+  Context {cont_preg: gen_heapGpreS N continuation_resource Σ}.
+  Context {exn_preg: gen_heapGpreS N exception Σ}.
+  Context {ghost_preg: ghostG Σ}.
+
+  Definition near_empty_store : store_record := Build_store_record [] [] [] [] [ ] [] [].
+
+  (* The following addresses could be generalised, as long as there are
+     no duplicates *)
+  Definition tag_exp_addr := 0%N.
+  Definition naturals_exp_addr := 1%N.
+  Definition sum_until_exp_addr := 4%N.
+
+  Definition mod_addr := 0%N.
+
+  
+  Definition exports: vi_store :=
+     (<[ tag_exp_addr := {| modexp_name := [Byte.x00]; modexp_desc := MED_global (Mk_globalidx (N.to_nat 0)) |} ]> (
+    (<[ naturals_exp_addr := {| modexp_name := [Byte.x00]; modexp_desc := MED_global (Mk_globalidx (N.to_nat 0)) |} ]> (
+      <[ sum_until_exp_addr := {| modexp_name := [Byte.x00]; modexp_desc := MED_global (Mk_globalidx (N.to_nat 0)) |} ]> ∅)))).
+  
+  Lemma generator_client_adequacy n he' S' V' M' HA':
+    rtc erased_step (([ (sum_until_client tag_exp_addr naturals_exp_addr sum_until_exp_addr mod_addr n, [], empty_frame) ],
+                       (near_empty_store, exports, [generator_module], [] )) : cfg wasm_host_lang)
+      ([he'] , (S', V', M', HA')) ->
+    (forall v, iris_host.to_val he' = Some v ->
+          v = (immHV [VAL_num (VAL_int32 $ Sum_until_i32 n)], empty_frame)).
+  Proof.
+    intros Hstep.
+    pose proof (wp_adequacy Σ wasm_host_lang NotStuck
+                  (sum_until_client tag_exp_addr naturals_exp_addr sum_until_exp_addr mod_addr n, [], empty_frame)
+                  (near_empty_store, exports, [generator_module], [] )
+                  (λ v,   v = (immHV [VAL_num (VAL_int32 $ Sum_until_i32 n)], empty_frame) 
+      )).
+    simpl in H.
+    
+    eassert _.
+    { apply H.
+      iIntros (Hinv κs).
+      iMod (gen_heap_init (∅:gmap N function_closure)) as (func_heapg) "[Hfunc_ctx _]".
+      iMod (gen_heap_init (∅:gmap (N*N) funcelem)) as (tab_heapg) "[Htab_ctx _]".
+      iMod (gen_heap_init (∅:gmap N nat)) as (tabsize_heapg) "[Htabsize_ctx _]".
+      iMod (@gen_heap_init _ _ _ _ _ tablimits_preg (∅:gmap N (option N))) as (tablimit_heapg) "[Htablimit_ctx _]".
+      iMod (gen_heap_init (∅:gmap (N*N) byte)) as (mem_heapg) "[Hmem_ctx _]".
+      iMod (gen_heap_init (∅:gmap N N)) as (memsize_heapg) "[Hmemsize_ctx _]".
+      iMod (@gen_heap_init _ _ _ _ _ memlimit_preg (∅:gmap N (option N))) as (memlimit_heapg) "[Hmemlimit_ctx _]".
+      iMod (gen_heap_init (∅:gmap N global)) as (global_heapg) "[Hglobal_ctx _]".
+      iMod (gen_heap_init (∅: gmap N function_type)) as (tag_heapg) "[Htag_ctx _]".
+      iMod (gen_heap_init (∅: gmap N continuation_resource)) as (cont_heapg) "[Hcont_ctx _]".
+      iMod (gen_heap_init (∅: gmap N exception)) as (exn_heapg) "[Hexn_ctx _]".
+      
+      apply (@gen_heapGpreS_heap) in vis_preg as vis_heapg.
+      iMod (ghost_map_alloc (∅:gmap N module_export)) as (γvis) "[Hvis_ctx _]".
+      apply (@gen_heapGpreS_heap) in ms_preg as ms_heapg.
+      iMod (ghost_map_alloc (∅:gmap N module)) as (γms) "[Hms_ctx _]".
+      apply (@gen_heapGpreS_heap) in has_preg as has_heapg.
+      iMod (ghost_map_alloc (∅:gmap N host_action)) as (γhas) "[Hhas_ctx _]".
+
+      iMod (@na_alloc Σ na_invg) as (logrel_nais) "Hna".
+      pose wasmg := WasmG Σ Hinv func_heapg cont_heapg exn_heapg tag_heapg tab_heapg tabsize_heapg
+                          tablimit_heapg mem_heapg memsize_heapg memlimit_heapg
+                          global_heapg.
+      pose visgg := HVisG Σ vis_heapg γvis.
+      pose msgg := HMsG Σ ms_heapg γms.
+      pose hasgg := HAsG Σ has_heapg γhas.
+      pose logrel_na_invs := Build_logrel_na_invs _ na_invg logrel_nais.
+
+      iMod (ghost_map_insert sum_until_exp_addr {| modexp_name := [Byte.x00]; modexp_desc := MED_global (Mk_globalidx (N.to_nat 0)) |}
+             with "Hvis_ctx") as "[Hvis_ctx Hv1]";[auto|].
+      iMod (ghost_map_insert naturals_exp_addr {| modexp_name := [Byte.x00]; modexp_desc := MED_global (Mk_globalidx (N.to_nat 0)) |}
+             with "Hvis_ctx") as "[Hvis_ctx Hv2]";[auto|].
+      iMod (ghost_map_insert tag_exp_addr {| modexp_name := [Byte.x00]; modexp_desc := MED_global (Mk_globalidx (N.to_nat 0)) |}
+             with "Hvis_ctx") as "[Hvis_ctx Hv3]";[auto|].
+      iMod (ghost_map_insert mod_addr generator_module with "Hms_ctx") as "[Hms_ctx Hm0]";[auto|].
+      
+      iDestruct (instantiate_client $! (λ v, ⌜ v = (immHV [VAL_num (VAL_int32 $ Sum_until_i32 n)], empty_frame) ⌝%I) 
+                  with "[$Hm0 Hv1 Hv2 Hv3]") as "HH".
+      iFrame. 
+
+      iDestruct ("HH" with "[]") as "HH";[auto|].
+      iModIntro.
+      iExists _,_.
+      iFrame "HH".
+      iFrame.
+    }
+    intros v Hval.
+    destruct X. eapply adequate_result with (t2 := []).
+    apply iris_host.of_to_val in Hval as <-. eauto.
+  Qed.
+
+End generator_client_adequacy.
+
+Theorem generalor_example:
+  forall n he' S' V' M' HA',
+    rtc erased_step (([ (sum_until_client tag_exp_addr naturals_exp_addr sum_until_exp_addr mod_addr n, [], empty_frame) ],
+                       (near_empty_store, exports, [generator_module], [] )) : cfg wasm_host_lang)
+      ([he'] , (S', V', M', HA')) ->
+    (forall v, iris_host.to_val he' = Some v ->
+          v = (immHV [VAL_num (VAL_int32 $ Sum_until_i32 n)], empty_frame)).
+Proof.
+   set (Σ := #[invΣ;
+              na_invΣ;
+              gen_heapΣ N function_closure;
+              gen_heapΣ (N*N) funcelem;
+              gen_heapΣ N nat;
+              gen_heapΣ N (option N);
+              gen_heapΣ (N*N) byte;
+              gen_heapΣ N N;
+              gen_heapΣ N (option N);
+              gen_heapΣ N global;
+              gen_heapΣ N module_export;
+              gen_heapΣ N module;
+               gen_heapΣ N host_action;
+               gen_heapΣ N function_type;
+               gen_heapΣ N continuation_resource;
+               gen_heapΣ N exception;
+               ghostΣ
+      ]).
+  eapply (@generator_client_adequacy Σ); typeclasses eauto.
+Qed.
+
